@prefix rdf:  <http://www.w3.org/1999/02/22-rdf-syntax-ns#> .
@prefix rdfs: <http://www.w3.org/2000/01/rdf-schema#> .
@prefix owl:  <http://www.w3.org/2002/07/owl#> .
@prefix onsgit: <https://github.com/ONS-OpenData/> .
@prefix cogs: <http://gss-cogs.uk/def/arch/> .

<http://gss-cogs.uk/def/arch> a owl:Ontology;
  rdfs:label "COGS Architecture" ;
.

cogs:SoftwarePackage a owl:Class ;
  rdfs:label "Software package" ;
.

cogs:PythonPackage a owl:Class ;
  rdfs:subClassOf cogs:SoftwarePackage ;
  rdfs:label "Python package" ;
.

onsgit:gss-utils a cogs:PythonPackage ;
  rdfs:label "gss-utils" ;
  rdfs:comment "Shared data transformation\nutilities for GSS data" ;
  cogs:requires onsgit:databaker ;
  cogs:requires <https://pandas.pydata.org> ;
.

<https://pandas.pydata.org> a cogs:PythonPackage ;
  rdfs:label "Pandas";
.

onsgit:databaker a cogs:PythonPackage ;
  rdfs:label "Databaker";
  rdfs:comment "ONS-OpenData fork";
.

cogs:JenkinsPipeline a owl:Class ;
  rdfs:label "Jenkins Pipeline" ;
.

cogs:TemplateJenkinsPipeline rdfs:subClassOf cogs:JenkinsPipeline;
  cogs:source <https://git.floop.org.uk/ONS/pmd-jenkins-library/blob/master/vars/transformPipeline.groovy> ;
  cogs:pipelineStep cogs:templateStep_clean, cogs:templateStep_transform, cogs:templateStep_validate, cogs:templateStep_upload, cogs:templateStep_test, cogs:templateStep_publish ;
.

cogs:DockerImage a owl:Class ;
  rdfs:label "Docker Image" ;
.

cogs:DockerContainer a owl:Class ;
  rdfs:label "Docker Container" ;
.

onsgit:csv2rdf-docker a cogs:DockerImage ;
  rdfs:label "CSV2RDF" ;
  rdfs:comment "Bundles Swrirrl's csv2rdf Clojure implementation for running in a Docker container."@en ;
  cogs:requires <https://github.com/Swirrl/csv2rdf> ;
.


cogs:ClojureLibrary a owl:Class ;
  rdfs:subClassOf cogs:SoftwarePackage ;
  rdfs:label "Clojure Library";
.

<https://github.com/Swirrl/csv2rdf> a cogs:ClojureLibrary ;
  rdfs:label "csv2rdf.clj" ;
  rdfs:comment "Swirrl's implementation of W3C CSVW specification.";
.


cogs:JenkinsPlugin a owl:Class ;
  rdfs:subClassOf cogs:SoftwarePackage ;
  rdfs:label "Jenkins Plugin" ;
.

<https://git.floop.org.uk/git/ONS/pmd-jenkins-library.git> a cogs:JenkinsPlugin ;
  rdfs:label "PMD Jenkins shared library" ;
.

onsgit:databaker-docker a cogs:DockerImage ;
  rdfs:label "cloudfluff/databaker" ;
  rdfs:comment "Databaker, Jupyter, Pandas and other tools";
  cogs:requires onsgit:databaker, <https://pandas.pydata.org>, onsgit:gss-utils ;
.

onsgit:csvlint-docker a cogs:DockerImage ;
  rdfs:label "cloudfluff/csvlint" ;
  rdfs:comment "Bundles the forked csvlint Ruby app in Docker for use in Jenkins Pipeline steps." ;
  cogs:requires onsgit:csvlint ;
.

cogs:RubyLibrary a owl:Class ;
  rdfs:subClassOf cogs:SoftwarePackage ;
  rdfs:label "Ruby Library" ;
.

onsgit:csvlint a cogs:RubyLibrary ;
  rdfs:label "csvlint.rb" ;
  rdfs:comment "Fork of ODS csvlint Ruby app for validating CSVW" ;
.

cogs:WebApp a owl:Class ;
  rdfs:subClassOf cogs:SoftwarePackage ;
  rdfs:label "Web app";
.

<https://git.floop.org.uk/git/ONS/csvlint-webapp.git> a cogs:WebApp ;
  rdfs:label "csvlint-webapp" ;
  rdfs:comment "Trivial Ruby web application, bundled in Docker, to validate given CSVW (CSV and JSON) files." ;
  cogs:requires onsgit:csvlint ;
.

<https://git.floop.org.uk/git/alex/sparql-test-runner.git> a cogs:DockerImage ;
  rdfs:label "sparql-test-runner" ;
  rdfs:comment "Runs a suite of queries-as-tests." ;
.

onsgit:gdp-sparql-tests a cogs:DockerImage ;
  rdfs:label "GDP ICs" ;
  rdfs:comment "Tests data against RDF Data Cube and PMD integrity constraints.";
  cogs:requires <https://git.floop.org.uk/git/alex/sparql-test-runner.git> ;
.

<https://git.floop.org.uk/git/ONS/jenkins-trello.git> a cogs:JenkinsPlugin ;
  rdfs:label "Trello updater" ;
  rdfs:comment "Jenkins plugin to update Trello card with current build state." ;
.

<https://git.floop.org.uk/git/ONS/jupyterhub.git> a cogs:WebApp ;
  rdfs:label "COGS JupyterHub" ;
  rdfs:comment "docker-compose based setup of the JupyterHub web application. Authenticates via github and spawns a container for each user.";
.