@prefix rdf:  <http://www.w3.org/1999/02/22-rdf-syntax-ns#> .
@prefix rdfs: <http://www.w3.org/2000/01/rdf-schema#> .
@prefix owl:  <http://www.w3.org/2002/07/owl#> .
@prefix cogsgit: <https://github.com/GSS-Cogs/> .
@prefix cogs: <http://gss-cogs.uk/def/arch/> .

<http://gss-cogs.uk/def/arch> a owl:Ontology;
  rdfs:label "COGS Architecture" ;
.

cogs:SoftwarePackage a owl:Class ;
  rdfs:label "Software package" ;
.
cogs:LandingPage a owl:Class ;
  rdfs:subClassOf cogs:SoftwarePackage ;
  rdfs:label "Original Data" ;
.
cogs:Datasets a owl:Class ;
  rdfs:subClassOf cogs:SoftwarePackage ;
  rdfs:label "Output Datasets" ;
.
cogs:Sheets a owl:Class ;
  rdfs:subClassOf cogs:SoftwarePackage ;
  rdfs:label "Sheets";
.
cogs:Columns a owl:Class ;
  rdfs:subClassOf cogs:SoftwarePackage ;
  rdfs:label "Columns" ;
.

cogs:splits_into a owl:ObjectProperty ;
  rdfs:subPropertyOf cogs:action ;
  rdfs:label "splits into" ;
  cogs:vis cogs:edge ;
.
cogs:transforms_into a owl:ObjectProperty ;
  rdfs:subPropertyOf cogs:action ;
  rdfs:label "transforms into" ;
  cogs:vis cogs:edge ;
.
cogs:outputs_columns a owl:ObjectProperty ;
  rdfs:subPropertyOf cogs:action ;
  rdfs:label "outputs columns" ;
  cogs:vis cogs:edge ;
.
###########################################################################################################

cogsgit:top-level a cogs:LandingPage ;
  rdfs:label "Statutory Homelessness detailed Local Authority-Level" ;
  rdfs:comment "https://www.gov.uk/government/statistical-data-sets/live-tables-on-homelessness";
  cogs:splits_into cogsgit:sheet1, cogsgit:sheet2, cogsgit:sheet3, cogsgit:sheet4 ;
.

cogsgit:sheet1 a cogs:Sheets ;
  rdfs:label "" ;
  rdfs:comment "A1, A2, A3, A4, A5P, A5R, A7, A11" ;
  cogs:transforms_into cogsgit:dataset1 ;
.
cogsgit:sheet2 a cogs:Sheets ;
  rdfs:label "" ;
  rdfs:comment "P1, P2, R1, R2" ;
  cogs:transforms_into cogsgit:dataset2 ;
.
cogsgit:sheet3 a cogs:Sheets ;
  rdfs:label "" ;
  rdfs:comment "MD1, MD2, MD3" ;
  cogs:transforms_into cogsgit:dataset3 ;
.
cogsgit:sheet4 a cogs:Sheets ;
  rdfs:label "" ;
  rdfs:comment "TA1, TA2" ;
  cogs:transforms_into cogsgit:dataset4 ;
.

cogsgit:dataset1 a cogs:Datasets ;
  rdfs:label "" ;
  rdfs:comment "MHCLG Homelessness - Households initially assessed as threatened with homelessness (owed prevention duty) or homeless (owed relief duty)" ;
  cogs:outputs_columns cogsgit:columns1 ;
.
cogsgit:dataset2 a cogs:Datasets ;
  rdfs:label "" ;
  rdfs:comment "MHCLG Homelessness - Households whose prevention or relief duty ended by reason and accommodation type" ;
  cogs:outputs_columns cogsgit:columns2 ;
.
cogsgit:dataset3 a cogs:Datasets ;
  rdfs:label "" ;
  rdfs:comment "MHCLG - Households assessed, following relief duty end, as unintentionally homeless and priority need (owed main duty)" ;
  cogs:outputs_columns cogsgit:columns3 ;
.
cogsgit:dataset4 a cogs:Datasets ;
  rdfs:label "" ;
  rdfs:comment "MHCLG Homelessness - Households in temporary accommodation by household composition and accommodation type" ;
  cogs:outputs_columns cogsgit:columns4 ;
.

cogsgit:columns1 a cogs:Columns ;
  rdfs:label "" ;
  rdfs:comment "Period, Accommodation Type, Household Composition, Initial Assessment, Reason for loss or threat of loss of home, Support needs of household, Duty Owed, Referral Public Body, Eligibility for Homelessness Status" ;
.
cogsgit:columns2 a cogs:Columns ;
  rdfs:label "" ;
  rdfs:comment "ONS Geography Code, Period, Accommodation Type, Reason duty Ended, Duty Type" ;
.
cogsgit:columns3 a cogs:Columns ;
  rdfs:label "" ;
  rdfs:comment "ONS Geography Code, Period, Decision on Duty Owed, Reason duty Ended, Priority Need" ;
.
cogsgit:columns4 a cogs:Columns ;
  rdfs:label "" ;
  rdfs:comment "ONS Geography Code, Period, Accommodation Type, Household Composition" ;
.
###################################################################################################
