@prefix rdf:  <http://www.w3.org/1999/02/22-rdf-syntax-ns#> .
@prefix rdfs: <http://www.w3.org/2000/01/rdf-schema#> .
@prefix owl:  <http://www.w3.org/2002/07/owl#> .
@prefix cogsgit: <https://github.com/GSS-Cogs/> .
@prefix cogs: <http://gss-cogs.uk/def/arch/> .

<http://gss-cogs.uk/def/arch> a owl:Ontology;
  rdfs:label "COGS Architecture" ;
.

cogs:vis a owl:AnnotationProperty ;
  rdfs:label "visualise as" ;
.

cogs:style a owl:Annotation ;
  rdfs:label "style" ;
.

cogs:container a owl:Annotation ;
  rdfs:label "contained by" ;
.

cogs:node a owl:Thing .
cogs:edge a owl:Thing .

cogs:Process a owl:Class ;
  rdfs:label "Process" ;
.

cogs:action a owl:ObjectProperty ;
  rdfs:label "Action" ;
.

cogs:Resource a owl:Class ;
  rdfs:label "Resource" ;
.

cogs:Container a owl:Class ;
  rdfs:label "Container" ;
.

:PMD a cogs:Container ;
  rdfs:label "Publish my Data" ;
  cogs:vis cogs:node ;
  cogs:style "fill: #dddddd; stroke: #999" ;
.

:table2qb a cogs:Container ;
  rdfs:label "table2qb" ;
  cogs:container :PMD ;
  cogs:vis cogs:node ;
  cogs:style "fill: #bbbbbb; stroke: #999;" ;
.

:table2qb_cube a cogs:Process ;
  rdfs:label "cube-pipeline" ;
  rdfs:comment "Generates cube RDF for the given input CSV and columns configuration." ;
  cogs:container :table2qb ;
  cogs:vis cogs:node ;
  cogs:generates :data_cube ;
.

:columns_csv a cogs:Resource ;
  rdfs:label "columns.csv" ;
  rdfs:comment "Map from column names to RDF dimensions and values" ;
  cogs:vis cogs:node ;
  cogs:input_to :table2qb_cube ;
  cogs:container :github_ref ;
.

:observations_csv a cogs:Resource ;
  rdfs:label "observations.csv" ;
  rdfs:comment "Tidy Data: one row per observation, one column per dimension." ;
  cogs:vis cogs:node ;
  cogs:input_to :table2qb_cube, :csvlint ;
  cogs:container :jenkins_pipeline ;
.

cogs:generates a owl:ObjectProperty ;
  rdfs:subPropertyOf cogs:action ;
  rdfs:label "generates" ;
  cogs:vis cogs:edge ;
.

cogs:input_to a owl:ObjectProperty ;
  rdfs:subPropertyOf cogs:action ;
  rdfs:label "input" ;
  cogs:vis cogs:edge;
.

cogs:refers_to a owl:ObjectProperty ;
  rdfs:subPropertyOf cogs:action ;
  rdfs:label "refers to" ;
  cogs:vis cogs:edge ;
.

:jupyter_transform a cogs:Process ;
  rdfs:label "Spreadsheet transform" ;
  rdfs:comment "A Jupyter notebook using Databaker, Pandas and gss-utils to convert a spreadsheet to Tidy data.";
  cogs:vis cogs:node ;
  cogs:generates :observations_csv, :observations_schema ;
  cogs:container :jenkins_pipeline ;
.

:data_cube a cogs:Resource ;
  rdfs:label "Data Cube" ;
  cogs:vis cogs:node ;
  cogs:container :PMD ;
  cogs:refers_to :components ;
  cogs:refers_to :codelists ;
.

#:jenkins_upload a cogs:Process ;
#  rdfs:label "Upload to PMD" ;
#  cogs:vis cogs:node ;
#  cogs:container :jenkins_pipeline ;
#.

:jenkins_pipeline a cogs:Container ;
  rdfs:label "Jenkins Pipeline" ;
  cogs:vis cogs:node ;
  cogs:style "fill: #aaaaee; stroke: #999;" ;
.

:github_ref a cogs:Container ;
  rdfs:label "Reference data" ;
  cogs:vis cogs:node ;
  cogs:style "fill: #444; stroke: aaa;" ;
.

:components_csv a cogs:Resource ;
  rdfs:label "components.csv" ;
  cogs:vis cogs:node ;
  cogs:container :github_ref ;
  cogs:input_to :table2qb_comp ;
.

:table2qb_comp a cogs:Process ;
  rdfs:label "components-pipeline" ;
  rdfs:comment "Generates RDF for the given components CSV file." ;
  cogs:container :table2qb ;
  cogs:vis cogs:node ;
  cogs:generates :components ;
.

:components a cogs:Resource ;
  rdfs:label "Components definitions" ;
  rdfs:comment "Definitions of dimensions, attributes and measures." ;
  cogs:vis cogs:node ;
  cogs:container :PMD ;
.

:codelists_csv a cogs:Resource ;
  rdfs:label "Codelists" ;
  rdfs:comment "A series of CSV files declaring hierarchical codelists that map codes to labels." ;
  cogs:vis cogs:node ;
  cogs:container :github_ref ;
  cogs:input_to :table2qb_codelist ;
.

:table2qb_codelist a cogs:Process ;
  rdfs:label "codelist-pipeline" ;
  rdfs:comment "Generates RDF for the given codelist CSV file" ;
  cogs:vis cogs:node ;
  cogs:container :table2qb ;
  cogs:generates :codelists ;
.

:codelists a cogs:Resource ;
  rdfs:label "Codelists" ;
  rdfs:comment "A series of SKOS Concept Schemes." ;
  cogs:vis cogs:node ;
  cogs:container :PMD ;
.

:csvlint a cogs:Process ;
  rdfs:label "csvlint" ;
  rdfs:comment "Validates CSV against a schema constraints including primary and foreign keys." ;
  cogs:vis cogs:node ;
  cogs:container :jenkins_pipeline ;
  cogs:refers_to :codelists_csv ;
.

:observations_schema a cogs:Resource ;
  rdfs:label "observations.csv-schema.json" ;
  cogs:vis cogs:node ;
  cogs:container :jenkins_pipeline ;
  cogs:input_to :csvlint ;
.