@prefix rdf:  <http://www.w3.org/1999/02/22-rdf-syntax-ns#> .
@prefix rdfs: <http://www.w3.org/2000/01/rdf-schema#> .
@prefix owl:  <http://www.w3.org/2002/07/owl#> .
@prefix cogsgit: <https://github.com/GSS-Cogs/> .
@prefix cogs: <http://gss-cogs.uk/def/arch/> .

<http://gss-cogs.uk/def/arch> a owl:Ontology;
  rdfs:label "COGS Homelessness Transform Mapping" ;
.

cogs:SoftwarePackage a owl:Class ;
  rdfs:label "Software package" ;
.
cogs:LandingPage a owl:Class ;
  rdfs:subClassOf cogs:SoftwarePackage ;
  rdfs:label "Landing Page" ;
.
cogs:Datasets a owl:Class ;
  rdfs:subClassOf cogs:SoftwarePackage ;
  rdfs:label "Output Dataset" ;
.
cogs:Sheets a owl:Class ;
  rdfs:subClassOf cogs:SoftwarePackage ;
  rdfs:label "Sheet names to join";
.
cogs:Columns a owl:Class ;
  rdfs:subClassOf cogs:SoftwarePackage ;
  rdfs:label "Table" ;
.
cogs:PMD a owl:Class ;
  rdfs:subClassOf cogs:SoftwarePackage ;
  rdfs:label "PMD" ;
.
###########################################################################################################

cogsgit:top-level a cogs:LandingPage ;
  rdfs:label "Homelessness in Scotland:  Equalities Breakdown" ;
  rdfs:comment "https://www2.gov.scot/Topics/Statistics/Browse/Housing-Regeneration/RefTables#Publications";
  cogs:splits cogsgit:sheet1, cogsgit:sheet2, cogsgit:sheet3 ;
.

cogsgit:sheet1 a cogs:Sheets ;
  rdfs:label "" ;
  rdfs:comment "Table 1, Table 2, Table 3, Table 4, Table 5, Table 6, Table 7, Table 8, Table 9, Table 10" ;
  cogs:transforms cogsgit:dataset1 ;
.
cogsgit:sheet2 a cogs:Sheets ;
  rdfs:label "" ;
  rdfs:comment "Table 11, Table 12, Table 13, Table 14, Table 15, Table 16, Table 17" ;
  cogs:transforms cogsgit:dataset2 ;
.
cogsgit:sheet3 a cogs:Sheets ;
  rdfs:label "" ;
  rdfs:comment "Table 18, Table 19" ;
  cogs:transforms cogsgit:dataset3 ;
.


cogsgit:dataset1 a cogs:Datasets ;
  rdfs:label "" ;
  rdfs:comment "SG -  Homelessness Equalities Breakdown - Applications & Assessments" ;
  cogs:outputs cogsgit:columns1 ;
.
cogsgit:dataset2 a cogs:Datasets ;
  rdfs:label "" ;
  rdfs:comment "SG -  Homelessness Equalities Breakdown - Temporary Accommodation" ;
  cogs:outputs cogsgit:columns2 ;
.
cogsgit:dataset3 a cogs:Datasets ;
  rdfs:label "" ;
  rdfs:comment "SG -  Homelessness Equalities Breakdown - Assessment Outcomes" ;
  cogs:outputs cogsgit:columns3 ;
.


cogsgit:columns1 a cogs:Columns ;
  rdfs:label "" ;
  rdfs:comment "Period, Sex, Age, Ethnicity, Household Composition, Accommodation Type, Rough Sleeping Occurrence, Armed Forces Membership, Previous Application to LA, Reason for Application, Failing to maintain Accommodation reasons, Assessment Decision, Reassessed as Homeless within same Year, Identified Support Need, Measure Type, Unit, Marker, Value" ;
  cogs:uploads cogsgit:pmd1 ;
.
cogsgit:columns2 a cogs:Columns ;
  rdfs:label "" ;
  rdfs:comment "Period, Sex, Age, Ethnicity, Temporary Accommodation Breakdown, Household Composition, Placement Type, Number of Placements, Applications Refused, Measure Type, Unit, Marker, Value" ;
  cogs:uploads cogsgit:pmd1 ;
.
cogsgit:columns3 a cogs:Columns ;
  rdfs:label "" ;
  rdfs:comment "Period, Sex, Age, Ethnicity, Outcome Type, Post Assessment Contact, Measure Type, Unit, Marker, Value" ;
  cogs:uploads cogsgit:pmd1 ;
.

cogsgit:pmd1 a cogs:PMD ;
  rdfs:label "" ;
  rdfs:comment "Publish my Data: http://gss-data.org.uk/data/search" ;
.
###################################################################################################
