@prefix rdf:  <http://www.w3.org/1999/02/22-rdf-syntax-ns#> .
@prefix rdfs: <http://www.w3.org/2000/01/rdf-schema#> .
@prefix owl:  <http://www.w3.org/2002/07/owl#> .
@prefix cogsgit: <https://github.com/GSS-Cogs/> .
@prefix cogs: <http://gss-cogs.uk/def/arch/> .

<http://gss-cogs.uk/def/arch> a owl:Ontology;
  rdfs:label "COGS Homelessness Transform Mapping" ;
.

cogs:SoftwarePackage a owl:Class ;
  rdfs:label "Software package" ;
.
cogs:LandingPage a owl:Class ;
  rdfs:subClassOf cogs:SoftwarePackage ;
  rdfs:label "Landing Page" ;
.
cogs:Datasets a owl:Class ;
  rdfs:subClassOf cogs:SoftwarePackage ;
  rdfs:label "Output Dataset" ;
.
cogs:Sheets a owl:Class ;
  rdfs:subClassOf cogs:SoftwarePackage ;
  rdfs:label "Sheet names to join";
.
cogs:Columns a owl:Class ;
  rdfs:subClassOf cogs:SoftwarePackage ;
  rdfs:label "Table" ;
.
cogs:PMD a owl:Class ;
  rdfs:subClassOf cogs:SoftwarePackage ;
  rdfs:label "PMD" ;
.
###########################################################################################################

cogsgit:top-level a cogs:LandingPage ;
  rdfs:label "Homelessness in Scotland: Annual Publication" ;
  rdfs:comment "https://www2.gov.scot/Topics/Statistics/Browse/Housing-Regeneration/RefTables#Publications";
  cogs:splits cogsgit:sheet1, cogsgit:sheet2, cogsgit:sheet3, cogsgit:sheet4 ;
.

cogsgit:sheet1 a cogs:Sheets ;
  rdfs:label "" ;
  rdfs:comment "Table 1, Table 2, Table 3, Table 4, Table 5, Table 6, Table 7, Table 8, Table 9, Table 10" ;
  cogs:transforms cogsgit:dataset1 ;
.
cogsgit:sheet2 a cogs:Sheets ;
  rdfs:label "" ;
  rdfs:comment "Table 11, Table 12, Table 13, Table 14, Table 15, Table 16" ;
  cogs:transforms cogsgit:dataset2 ;
.
cogsgit:sheet3 a cogs:Sheets ;
  rdfs:label "" ;
  rdfs:comment "Table 17, Table 18, Table 19, Table 20, Table 21, Table 22, Table 23, Table 24, Table 25, Table 26, Table 27, Table 28, Table 29" ;
  cogs:transforms cogsgit:dataset3 ;
.
cogsgit:sheet4 a cogs:Sheets ;
  rdfs:label "" ;
  rdfs:comment "Table 30, Table 31, Table 32, Table 33" ;
  cogs:transforms cogsgit:dataset4 ;
.

cogsgit:dataset1 a cogs:Datasets ;
  rdfs:label "" ;
  rdfs:comment "SG - Homelessness Applications Annual Publication" ;
  cogs:outputs cogsgit:columns1 ;
.
cogsgit:dataset2 a cogs:Datasets ;
  rdfs:label "" ;
  rdfs:comment "SG - Homelessness Assessment Decisions Annual Publication" ;
  cogs:outputs cogsgit:columns2 ;
.
cogsgit:dataset3 a cogs:Datasets ;
  rdfs:label "" ;
  rdfs:comment "SG - Homelessness Temporary Accommodation Annual Publication" ;
  cogs:outputs cogsgit:columns3 ;
.
cogsgit:dataset4 a cogs:Datasets ;
  rdfs:label "" ;
  rdfs:comment "SG - Homelessness Assessment Outcomes Annual Publication" ;
  cogs:outputs cogsgit:columns4 ;
.

cogsgit:columns1 a cogs:Columns ;
  rdfs:label "" ;
  rdfs:comment "Period, ONS Geography Code, Rough Sleeping Occurrence, Accommodation type, Homelessness Breakdown, Armed Forces Membership, Previous Application to LA, Sex, Age, Household Composition, Ethnicity, Reason for Application, Failing to maintain Accommodation reasons, Measure Type, Unit, Marker, Value" ;
  cogs:uploads cogsgit:pmd1 ;
.
cogsgit:columns2 a cogs:Columns ;
  rdfs:label "" ;
  rdfs:comment "Period, ONS Geography Code, Assessment Decision, Identified Support Need, Measure Type, Unit, Marker, Value	" ;
  cogs:uploads cogsgit:pmd1 ;
.
cogsgit:columns3 a cogs:Columns ;
  rdfs:label "" ;
  rdfs:comment "Period, ONS Geography Code, Accommodation type, Household Composition, Temporary Accommodation Breakdown, Placement Type, Measure Type, Unit, Marker, Value" ;
  cogs:uploads cogsgit:pmd1 ;
.
cogsgit:columns4 a cogs:Columns ;
  rdfs:label "" ;
  rdfs:comment "Period, ONS Geography Code, Outcome Type, Assessment Decision, Post Assessment Contact, Measure Type, Unit, Marker, Value" ;
  cogs:uploads cogsgit:pmd1 ;
.

cogsgit:pmd1 a cogs:PMD ;
  rdfs:label "" ;
  rdfs:comment "Publish my Data: http://gss-data.org.uk/data/search" ;
.
###################################################################################################
